src/coq/Handlers/SerializationTheory.v
@@ -10,6 +10,7 @@ From Vellvm Require Import
      Utils.ListUtil
      Utils.Error
      Utils.RefineProp
+     Utils.Monads
      Handlers.MemoryModelImplementation
      Handlers.Serialization
      Semantics.LLVMEvents
